
\documentclass{article}

\usepackage{amsmath}

\setcounter{MaxMatrixCols}{10}

\newcommand{\tab}{\hspace{5mm}}
\input{tcilatex}

\begin{document}



Fine structure constant:

$\alpha =\dfrac{e^{2} }{\left( 4\pi \varepsilon _{0} \right) \hbar c} $%
Length:\newline
Bohr radius:

\begin{eqnarray*}
a_{0} & = & \left( 4\pi \varepsilon _{0} \right) \dfrac{\hbar ^{2} }{m_{e}
e^{2} } \\
& = & \left[ \left( \dfrac{4\pi \varepsilon _{0} }{e^{2} } \right) \hbar c%
\right] \dfrac{\hbar }{m_{e} c} \\
& = & \dfrac{1}{\alpha } \left( \dfrac{\hbar }{m_{e} c} \right)
\end{eqnarray*}
CityplaceCompton wavelength:

$\lambdabar _{c} =\alpha a_{0} $Classical radius of the electron:

$R_{e} \approx \alpha ^{2} a_{0} $Bohr energy:

\begin{eqnarray*}
E_{n} & = & -\dfrac{1}{2} \left( \dfrac{e^{2} }{4\pi \varepsilon _{0} }
\right) ^{2} \left( \dfrac{m_{e} }{\hbar ^{2} } \right) \left( \dfrac{1}{%
n^{2} } \right) \\
& = & \left( \dfrac{e^{2} }{4\pi \varepsilon _{0} } \right) \left( \dfrac{1}{%
2n^{2} a_{0} } \right) \\
& = & -\dfrac{1}{2n^{2} } \alpha ^{2} m_{e} c^{2}
\end{eqnarray*}
Bohr magneton:

$\mu _{B} =\dfrac{e\hbar }{2m_{e} } $

Commutators:


\begin{equation*}
p\rightarrow \frac{\hbar }{i} \frac{d}{dx} \qquad\quad\;\;x\rightarrow -%
\frac{\hbar }{i} \frac{d}{dp} 
\end{equation*}

\begin{equation*}
\left( \Delta A\right) ^{2} \left( \Delta B\right) ^{2} \geq -\frac{1}{4}
\left\langle \left[ A,B\right] \right\rangle ^{2} 
\end{equation*}%
\newpage Harmonic oscillator:

\begin{equation*}
\alpha =\sqrt{\frac{m\omega }{\hbar } } 
\end{equation*}
\begin{gather*}
\hat{a} =\dfrac{1}{\sqrt{2} } \left( \alpha \hat{x} +i\dfrac{1}{\alpha \hbar 
} \hat{p} \right) =\text{lowering} \;\;\&\;\;\hat{a} ^{\dag } =\dfrac{1}{%
\sqrt{2} } \left( \alpha \hat{x} -i\dfrac{1}{\alpha \hbar } \hat{p} \right) =%
\text{raising} \\
\hat{x} =\dfrac{1}{\sqrt{2} \alpha } \left( \hat{a} +\hat{a} ^{\dag }
\right) \;\;\&\;\;\hat{p} =-i\dfrac{\alpha \hbar }{\sqrt{2} } \left( \hat{a}
-\hat{a} ^{\dag } \right)
\end{gather*}

$\hat{a} \left. n \right\rangle =\sqrt{n} \left. n-1 \right\rangle \;\;\&\;\;%
\hat{a} ^{\dag } \left. n \right\rangle =\sqrt{\left( n+1\right) } \left.
n+1 \right\rangle $ $\left[ \hat{a} ,\hat{a} ^{\dag } \right] =1$ $\hat{H}
=\hbar \omega \left( \hat{a} ^{\dag } \hat{a} +\dfrac{1}{2} \right) $ $\left[
\hat{H} ,\hat{a} \right] =-\hbar \omega \hat{a} \quad\;\;\,\left[ \hat{H} ,%
\hat{a} ^{\dag } \right] =\hbar \omega \hat{a} ^{\dag } $Let $\hat{x} =%
\dfrac{1}{\alpha } \hat{X} \;\;\&\;\;\hat{p} =\alpha \hbar \hat{P} $Which
leads to

$\hat{a} =\dfrac{1}{\sqrt{2} } \left( \hat{X} +i\hat{P} \right) \;\;\&\;\;%
\hat{a} ^{\dag } =\dfrac{1}{\sqrt{2} } \left( \hat{X} -i\hat{P} \right) $Also

$\hat{x} =\dfrac{1}{\sqrt{2} \alpha } \left( \hat{a} +\hat{a} ^{\dag }
\right) \;\;\&\;\;\hat{p} =-i\dfrac{\alpha \hbar }{\sqrt{2} } \left( \hat{a}
-\hat{a} ^{\dag } \right) $and

$\hat{X} =\dfrac{1}{\sqrt{2} } \left( \hat{a} +\hat{a} ^{\dag } \right)
\;\;\&\;\;\hat{P} =\dfrac{-i}{\sqrt{2} } \left( \hat{a} -\hat{a} ^{\dag }
\right) $Heisenberg picture -- harmonic oscillator:

\begin{eqnarray*}
\hat{x} \left( t\right) & = & \hat{x} \left( 0\right) \cos \omega t+\dfrac{%
\hat{p} \left( 0\right) }{m\omega } \sin \omega t \\
& = & \hat{x} \left( 0\right) \cos \omega t+\left( \dfrac{1}{\alpha ^{2}
\hbar } \right) \hat{p} \left( 0\right) \sin \omega t \\
\hat{p} \left( t\right) & = & \hat{p} \left( 0\right) \cos \omega t-m\omega 
\hat{x} \left( 0\right) \sin \omega t \\
& = & \hat{p} \left( 0\right) \cos \omega t-\left( \alpha ^{2} \hbar \right) 
\hat{x} \left( 0\right) \sin \omega t
\end{eqnarray*}

\begin{gather*}
\text{For\ the\ normalized\ Gaussian} \\
\psi \left( x\right) =\dfrac{\sqrt{\beta } }{\pi ^{1/4} } e^{-\beta ^{2}
x^{2} /2} \quad\;\;\Delta x=\dfrac{1}{\sqrt{2} \beta } \;\;\Rightarrow
\;\;\psi \left( x\right) =\dfrac{1}{\pi ^{1/4} } \left( \dfrac{1}{2^{1/4} 
\sqrt{\Delta x} } \right) e^{-x^{2} /\left( 4\Delta x^{2} \right) } \\
\text{For\ the\ Fourier\ transform\ of\ } \psi \left( x\right) \text{\
which\ is} \\
\phi \left( p\right) =\dfrac{1}{\pi ^{1/4} \sqrt{\beta \hbar } } e^{-p^{2}
/\left( 2\beta ^{2} \hbar ^{2} \right) } \quad\;\;\Delta p=\dfrac{1}{\sqrt{2}
} \beta \hbar \;\;\Rightarrow \;\;\phi \left( p\right) =\dfrac{1}{\pi ^{1/4} 
} \left( \dfrac{1}{2^{1/4} \sqrt{\Delta p} } \right) e^{-p^{2} /\left(
4\Delta p^{2} \right) }
\end{gather*}

\end{document}
