
\documentclass{article}
\usepackage{amsmath}
                                                                                                    
                                                                                                    
\newcommand{\tab}{\hspace{5mm}}


\begin{document}


M-List


\begin{center}
Mechanics


\end{center}


Lagrange's Equations with Undetermined Multipliers:


\[\frac{d}{dt} \left( \frac{\partial L}{\partial \dot{q} _{j} } \right)
-\frac{\partial L}{\partial q_{j} } =\sum\limits_{k}\lambda _{k} \left(
t\right) \frac{\partial f_{k} }{\partial q_{j} }  
\]


\[ \;\;;\;\;\dot{p}
_{j} \equiv \frac{\partial L}{\partial q_{j} } 
\] \begin{gather*}
 \\
 \\
-\frac{\partial H}{\partial t} =\frac{\partial L}{\partial t} 
\end{gather*}

Orbit equation for a known orbit 

\[r=r\left( \theta \right) 



\[\frac{d^{2} }{d\theta ^{2} } \left( \frac{1}{r} \right) +\frac{1}{r}
=-\frac{\mu r^{2} }{l^{2} } F\left( r\right) 
\]where 
\[\mu \equiv \frac{m_{1} m_{2} }{m_{1} +m_{2} } 
\], and 
\[l\equiv \mu r^{2} \dot{\theta } =\text{constant} 
\]


\[E=\frac{1}{2} \mu \dot{r} ^{2} +\frac{1}{2} \frac{l^{2} }{\mu r^{2} }
+U\left( r\right) 
\]
\begin{center}
Electrodynamics


\end{center}

:


\[

Electric field of a system of point charges:


\[\vec{E} \left( \vec{r} \right) =\frac{1}{4\pi \epsilon _{0} }
\sum\limits_{i=1}^{n}\frac{q_{i} }{r_{i} ^{2} }  \hat{r} _{i} 
\]
Electric field for charge distributions:


\[\vec{E} \left( \vec{r} \right) =\frac{1}{4\pi \epsilon _{0} } \int
\frac{\rho \left( \vec{r} ^{'} \right) }{r^{2} }  \hat{r} d\tau ^{'} 
\]
Gauss's Law:


\[\Phi _{E} =\int\limits_{S}\vec{E} \cdot d\vec{a}  =\frac{1}{\epsilon _{0}
} Q_{enc} 
\]
\[\Phi _{B} =\oint\nolimits_{S}\vec{B} \cdot d\vec{a}
=\oint\nolimits_{S}\nabla \times \vec{A} \cdot d\vec{a}
=\oint\nolimits_{C}\vec{A} \cdot d\vec{l}    
\]
Solution to placeLaplace's Equation in spherical coordinates 
with no 
$\phi $ dependence:


\[V\left( r,\theta \right) =\sum\limits_{l=0}^{\infty }\left( A_{l} r^{l}
+B_{l} r^{-\left( l+1\right) } \right)  P_{l} \left( \cos \theta \right) 
\]
Solution to placeLaplace's Equation in cylindrical coordinates:


\[V\left( \rho ,\phi \right) =D_{0} +C_{0} \ln \rho
+\sum\limits_{n=1}^{\infty }\left[ A_{n} \cos \left( n\phi \right) +B_{n}
\sin \left( n\phi \right) \right]  \left( C_{n} \rho ^{-n} +D_{n} \rho
^{n} \right) 
\]
Maxwell's Equations: \\
In general:


\[\nabla \cdot \vec{E} =\frac{1}{\epsilon _{0} } \rho 
\]
\[\nabla \times \vec{E} =-\frac{\partial \vec{B} }{\partial t} 
\]
\[\nabla \cdot \vec{B} =0
\]
\[\nabla \times \vec{B} =\mu _{0} \vec{J} +\mu _{0} \epsilon _{0}
\frac{\partial \vec{E} }{\partial t} 
\]
 In matter:


\[\nabla \cdot \vec{D} =\rho _{f} 
\]
\[\nabla \times \vec{E} =-\frac{\partial \vec{B} }{\partial t} 
\]
\[\nabla \cdot \vec{B} =0
\]
\[\nabla \times \vec{H} =\vec{J} _{f} +\frac{\partial \vec{D} }{\partial t} 
\]
Potentials:


\[\vec{E} =-\nabla V-\frac{\partial \vec{A} }{\partial t} 
\], 
\[\vec{B} =\nabla \times \vec{A} 
\]


Lorentz force law:


\[\vec{F} =q\left( \vec{E} +\vec{v} \times \vec{B} \right) 
\]\newpage

\begin{center}
Quantum Mechanics


\end{center}

Classical Hamiltonian:


\[H\left( x,p\right) =\frac{p^{2} }{2m} +V\left( x\right) 
\]
for QM:


\[p\rightarrow \frac{\hbar }{i} \left( \frac{\partial }{\partial x} \right)
\quad;\;\,x\rightarrow -\frac{\hbar }{i} \left( \frac{\partial }{\partial
p} \right) 
\]
\[\hat{H} =-\frac{\hbar ^{2} }{2m} \frac{\partial ^{2} }{\partial x^{2} }
+V\left( x\right) 
\] $\hat{H} \psi =E\psi $
Particle in a box of length L, 0\texttt{<}x\texttt{<}L:


\[\frac{d^{2} \psi }{dx^{2} } =-k^{2} \psi 
\], 
\[k^{2} =\frac{2mE}{\hbar } 
\]


\[\psi _{n} \left( x\right) =A\sin \left( \frac{n\pi x}{L} \right) 
\], 
\[A=\sqrt{\frac{2}{L} } 
\]


\[E_{n} =\frac{n^{2} \pi ^{2} \hbar ^{2} }{2mL^{2} } 
\]
Particle in a box of length a, 

\[-\frac{a}{2} <x<\frac{a}{2} 
\]:


\[\frac{d^{2} \psi }{dx^{2} } =-k^{2} \psi 
\]\tab \tab 
\[k^{2} =\frac{2mE}{\hbar } 
\]\tab 
\[A=\sqrt{\frac{2}{L} } 
\]
\[\psi _{n} \left( x\right) =A\cos \left( \frac{n\pi x}{a} \right) 
\]\tab for odd n\tab 


\[\psi _{n} \left( x\right) =A\sin \left( \frac{n\pi x}{a} \right) 
\] for even n


QM harmonic oscillator:


\[a^{\dagger } \left| \right\rangle u_{n} =\sqrt{n+1} \left| \right\rangle
u_{n+1} 
\]
\[a^{} \left| \right\rangle u_{n} =\sqrt{n} \left| \right\rangle u_{n-1} 
\]
\[a^{\dagger } =\sqrt{\frac{m\omega }{2\hbar } } x-i\frac{p}{\sqrt{2m\hbar
\omega } } 
\]
\[a^{} =\sqrt{\frac{m\omega }{2\hbar } } x+i\frac{p}{\sqrt{2m\hbar \omega }
} 
\]
\[a^{\dagger } +a^{} =\sqrt{\frac{2m\omega }{\hbar } } x
\], let 
\[\alpha =\sqrt{\frac{m\omega }{\hbar } } 
\]


\[x=\dfrac{1}{\sqrt{2} \alpha } \left( a^{\dagger } +a\right) 
\]
Time-independent perturbation theory:


\[E_{n}^{1} =\left\langle \psi _{n}^{0} \left| H^{'} \right| \right. \left.
\psi _{n}^{0} \right\rangle 
\] (first order correction to energy)


Commutators:



\[\left[ x,p\right] =i\hbar 
\]

\[p\rightarrow \frac{\hbar }{i} \frac{d}{dx} \qquad\quad\;\;x\rightarrow
-\frac{\hbar }{i} \frac{d}{dp} 
\]

\[\left( \Delta A\right) ^{2} \left( \Delta B\right) ^{2} \geq -\frac{1}{4}
\left\langle \left[ A,B\right] \right\rangle ^{2} 
\]Harmonic oscillator: 

\[\alpha =\sqrt{\frac{m\omega }{\hbar } } 
\]


\begin{gather*}
\hat{a} =\dfrac{1}{\sqrt{2} } \left( \alpha \hat{x} +i\dfrac{1}{\alpha
\hbar } \hat{p} \right) \;\;\&\;\;\hat{a} ^{\dag } =\dfrac{1}{\sqrt{2} }
\left( \alpha \hat{x} -i\dfrac{1}{\alpha \hbar } \hat{p} \right)  \\
\hat{x} =\dfrac{1}{\sqrt{2} \alpha } \left( \hat{a} +\hat{a} ^{\dag }
\right) \;\;\&\;\;\hat{p} =-i\dfrac{\alpha \hbar }{\sqrt{2} } \left(
\hat{a} -\hat{a} ^{\dag } \right) 
\end{gather*}

$\left[ \hat{a} ,\hat{a} ^{\dag } \right] =1$
$\hat{H} =\hbar \omega \left( \hat{a} ^{\dag } \hat{a} +\dfrac{1}{2}
\right) $Let 
$\hat{x} =\dfrac{1}{\alpha } \hat{X} \;\;\&\;\;\hat{p} =\alpha \hbar
\hat{P} $Which leads to


$\hat{a} =\dfrac{1}{\sqrt{2} } \left( \hat{X} +i\hat{P} \right)
\;\;\&\;\;\hat{a} ^{\dag } =\dfrac{1}{\sqrt{2} } \left( \hat{X} -i\hat{P}
\right) $Also


$\hat{x} =\dfrac{1}{\sqrt{2} \alpha } \left( \hat{a} +\hat{a} ^{\dag }
\right) \;\;\&\;\;\hat{p} =-i\dfrac{\alpha \hbar }{\sqrt{2} } \left(
\hat{a} -\hat{a} ^{\dag } \right) $and


$\hat{X} =\dfrac{1}{\sqrt{2} } \left( \hat{a} +\hat{a} ^{\dag } \right)
\;\;\&\;\;\hat{P} =\dfrac{-i}{\sqrt{2} } \left( \hat{a} -\hat{a} ^{\dag }
\right) $
\[E_{n}^{2} =\sum\limits_{m\neq n}\frac{\left| \left\langle \psi _{m}^{0}
\right| H^{'} \left| \right\rangle \psi _{n}^{0} \right| ^{2} }{E_{n}^{0}
-E_{m}^{0} }  
\] (second order correction to energy)


\[\psi _{n}^{1} =\sum\limits_{m\neq n}\frac{\left\langle \psi _{m}^{0}
\left| H^{'} \right| \left. \psi _{n}^{0} \right\rangle \right. }{\left(
E_{n}^{0} -E_{m}^{0} \right) }  \psi _{m}^{0} 
\] (first order correction to the wave function\\



\begin{center}
Modern Physics


\end{center}

Relativity:


\[\gamma =\frac{1}{\sqrt{1-\frac{v^{2} }{c^{2} } } } =\frac{1}{\sqrt{1-\beta
^{2} } } ,\beta =\frac{v}{c} 
\]
\[t^{'} =\gamma \left( t-\frac{v}{c^{2} } x\right) 
\]
\[x^{'} =\gamma \left( x-vt\right) 
\]$m=\gamma m_{0} $
\[E=mc^{2} =\gamma m_{0} c^{2} 
\]
\[E^{2} =p^{2} c^{2} +m_{0}^{2} c^{4} 
\]$E=KE+m_{0} c^{2} $
\[KE=\left( \gamma -1\right) m_{0} c^{2} 
\]$p=\gamma m_{0} v$
\[L=\frac{L_{0} }{\gamma } 
\]
Hydrogen Atom:


\[E_{n} =\frac{-13.6eV}{n^{2} } =\frac{-1}{n^{2} } Ryd
\]

Treat excited one-electron atoms like Hydrogen, but include the 
effective charge, Z:


\[E_{n} =\frac{-13.6*Z^{2} }{n^{2} } =E_{n} (H_{2} )*Z^{2} 
\]


\end{document}
